src/3d/prelude/ResultOps.fst
@@ -60,14 +60,3 @@ let is_range_okay (size offset access_size:U32.t)
     size >=^ access_size &&
     size -^ access_size >=^ offset
 
-
-(* Context for default error handler *)
-
-noeq
-type error_frame = {
-  filled: bool;
-  start_pos: U32.t;
-  typename: string;
-  fieldname: string;
-  reason: string;
-}
